saving

basic_types.v
@@ -8,12 +8,22 @@ Definition oof M A: (@Syntax.judgement False) := deq M M A.
 
 Definition oof_t M: (@Syntax.judgement False) := deqtype M M.
 
+Definition U0 : (term False) := univ nzero.
+
+Definition leq_t n m : term False :=
+  app (app leqtp n) m.
+
 Lemma zero_typed: forall G,
     tr G (oof nzero nattp). Admitted.
 
 Lemma leq_refl: forall G n,
     tr G (deq n n nattp) ->
     tr G (oof triv (leqpagetp n n)). Admitted.
+
+Lemma leq_type: forall G n1 n2,
+    tr G (oof n1 nattp) -> tr G (oof n2 nattp) ->
+    tr G (oof (leq_t n1 n2) U0).
+  Admitted.
 
 Hint Resolve zero_typed.
 Hint Resolve leq_refl.
